Fix AllocationAlgo for mutual.

Coherence/AllocationAlgo.v
@@ -1,40 +1,87 @@
 Require Import CSet Le Arith.Compare_dec.
 
 Require Import Plus Util Map CMap Status.
-Require Import Val Var Env EnvTy IL Annotation Liveness Fresh Sim MoreList.
+Require Import Val Var Env EnvTy IL Annotation Liveness Fresh MoreList SetOperations.
 Require Import Coherence Allocation RenamedApart.
 
 Set Implicit Arguments.
 
 (** * SSA-based register assignment formulated for IL *)
 
-Fixpoint reg_assign (st:stmt) (an: ann (set var)) (ϱ:Map [var, var])
+
+Definition regAssignF
+           (regAssign : stmt -> ann (set var) -> Map [var, var] -> status (Map [var, var]))
+  := fix regAssignF
+           (ϱ:Map [var, var]) (F:list (list var * stmt)) (ans: list (ann (set var)))
+: status (Map [var, var]) :=
+  match F, ans with
+    | Zs::F, a::ans =>
+      let Z := fst Zs in let s := snd Zs in
+      let Z' := fresh_list least_fresh (SetConstructs.map (findt ϱ 0) (getAnn a\of_list Z)) (length Z) in
+      sdo ϱ' <- regAssign s a (ϱ[Z <-- Z']);
+        regAssignF ϱ' F ans
+
+    | nil, nil => Success ϱ
+    | _, _ => Error "regAssignF: function annotation mismatch"
+  end.
+
+Fixpoint regAssign (st:stmt) (an: ann (set var)) (ϱ:Map [var, var])
   : status (Map [var, var]) :=
  match st, an with
     | stmtLet x e s, ann1 lv ans =>
       let xv := least_fresh (SetConstructs.map (findt ϱ 0) (getAnn ans\{{x}})) in
-        reg_assign s ans (ϱ[x<- xv])
+        regAssign s ans (ϱ[x<- xv])
     | stmtIf _ s t, ann2 lv ans ant =>
-      sdo ϱ' <- reg_assign s ans ϱ;
-        reg_assign t ant ϱ'
+      sdo ϱ' <- regAssign s ans ϱ;
+        regAssign t ant ϱ'
     | stmtApp _ _, ann0 _ => Success ϱ
     | stmtReturn _, ann0 _ => Success ϱ
     | stmtExtern x f Y s, ann1 lv ans =>
       let xv := least_fresh (SetConstructs.map (findt ϱ 0) (getAnn ans\{{x}})) in
-      reg_assign s ans (ϱ[x<- xv])
-    | stmtFun Z s t, ann2 _ ans ant =>
-      let Z' := fresh_list least_fresh (SetConstructs.map (findt ϱ 0) (getAnn ans\of_list Z)) (length Z) in
-      sdo ϱ' <- reg_assign s ans (ϱ[Z <-- Z']);
-        reg_assign t ant ϱ'
-    | _, _ => Error "reg_assign: Annotation mismatch"
+      regAssign s ans (ϱ[x<- xv])
+    | stmtFun F t, annF _ ans ant =>
+      sdo ϱ' <- regAssignF regAssign ϱ F ans;
+        regAssign t ant ϱ'
+    | _, _ => Error "regAssign: Annotation mismatch"
  end.
 
 (** The algorithm only changes bound variables in the mapping [ϱ] *)
 
-Lemma reg_assign_renamedApart_agree' i s al ϱ ϱ' LV alv G
+Lemma regAssign_renamedApart_agreeF G F ans als ϱ ϱ'
+      (allocOK:regAssignF regAssign ϱ F als = Success ϱ')
+      (REN:forall (n : nat) (Zs : params * stmt) (a : ann (set var * set var)),
+             get F n Zs -> get ans n a -> renamedApart (snd Zs) a)
+      (LEN1:length F = length als)
+      (LEN2:length F = length ans)
+      (IH:(forall (n : nat) (Zs : params * stmt) (a : ann (set var)),
+             get F n Zs ->
+             get als n a ->
+             forall (al : ann (set var * set var)) (ϱ0 ϱ'0 : Map  [var, var])
+               (G0 : set var),
+               renamedApart (snd Zs) al ->
+               regAssign (snd Zs) a ϱ0 = Success ϱ'0 ->
+               agree_on eq (G0 \ snd (getAnn al)) (findt ϱ0 0) (findt ϱ'0 0)))
+: forall G' : set var,
+    list_union zip defVars F ans[<=]G' ->
+    agree_on eq (G \ G') (findt ϱ 0) (findt ϱ' 0).
+Proof.
+ intros G' INCL.
+ length_equify. general induction LEN1; inv LEN2; simpl in * |- *; try monadS_inv allocOK; eauto.
+ exploit IHLEN1; eauto using get. etransitivity; try eapply INCL.
+ norm_lunion. eauto with cset.
+ exploit IH; eauto using get.
+ rewrite <- map_update_list_update_agree in X1; eauto.
+ etransitivity; try eapply X0.
+ eapply agree_on_incl. eapply update_with_list_agree_inv; try eapply X1; eauto.
+ instantiate (1:=G). rewrite minus_union.
+ eapply incl_minus_lr; eauto.
+ erewrite <- INCL. norm_lunion. unfold defVars. eauto with cset.
+Qed.
+
+Lemma regAssign_renamedApart_agree' i s al ϱ ϱ' LV alv G
+      (allocOK:regAssign s alv ϱ = Success ϱ')
       (sd:renamedApart s al)
       (LS:live_sound i LV s alv)
-      (allocOK:reg_assign s alv ϱ = Success ϱ')
 : agree_on eq (G \ snd (getAnn al)) (findt ϱ 0) (findt ϱ' 0).
 Proof.
   general induction LS; inv sd; simpl in * |- *; try monadS_inv allocOK; eauto.
@@ -60,40 +107,154 @@ Proof.
     instantiate (1:=G).
     rewrite H11. simpl in *.
     revert H6; clear_all; cset_tac; intuition.
-  - exploit IHLS1; eauto.
-    exploit IHLS2; eauto.
-    rewrite <- map_update_list_update_agree in X.
-    rewrite H9 in X. rewrite H12 in X0. simpl in *.
-    etransitivity; try eapply X0.
-    eapply agree_on_incl. eapply update_with_list_agree_inv; try eapply X; eauto.
-    rewrite fresh_list_length; eauto.
-    instantiate (1:=G). rewrite <- H7.
-    revert H5; clear_all; cset_tac; intuition; eauto.
-    eapply agree_on_incl; eauto. instantiate (1:=G).
-    rewrite <- H7. clear_all; cset_tac; intuition; eauto.
-    rewrite fresh_list_length; eauto.
+  - exploit IHLS; eauto.
+    etransitivity; [| eapply agree_on_incl; try eapply X].
+    eapply agree_on_incl; try eapply regAssign_renamedApart_agreeF; eauto; try reflexivity.
+    rewrite <- H13. eapply incl_minus_lr; eauto; try reflexivity.
+    eapply incl_minus_lr; try reflexivity. rewrite <- H13. pe_rewrite; eauto with cset.
 Qed.
 
-Lemma reg_assign_renamedApart_agree i s al ϱ ϱ' LV alv
+Lemma regAssign_renamedApart_agree i s al ϱ ϱ' LV alv
       (sd:renamedApart s al)
       (LS:live_sound i LV s alv)
-      (allocOK:reg_assign s alv ϱ = Success ϱ')
+      (allocOK:regAssign s alv ϱ = Success ϱ')
 : agree_on eq (fst (getAnn al)) (findt ϱ 0) (findt ϱ' 0).
 Proof.
   eapply agree_on_incl.
-  eapply reg_assign_renamedApart_agree'; eauto.
+  eapply regAssign_renamedApart_agree'; eauto.
   instantiate (1:=fst (getAnn al)).
   exploit renamedApart_disj; eauto.
   revert X. unfold disj.
   clear_all; cset_tac; intuition; eauto.
 Qed.
 
+Fixpoint take n X (L:list X) :=
+  match n, L with
+    | S n, x::L => x::take n L
+    | _, _ => nil
+  end.
+
+Ltac eadmit := exfalso; clear_all; admit.
+
+Lemma regAssignF_get G F ans alv n Zs a ϱ ϱ' an Lv i D Dt lv
+: regAssignF regAssign ϱ F alv = Success ϱ'
+  -> (forall n Zs a, get F n Zs -> get ans n a -> renamedApart (snd Zs) a)
+  -> (forall n Zs a, get F n Zs ->
+               get alv n a ->
+               live_sound i Lv (snd Zs) a)
+  -> (forall (n : nat) (Zs : params * stmt) (a : ann (set var)),
+       get F n Zs ->
+       get alv n a ->
+       of_list (fst Zs)[<=]getAnn a /\ getAnn a \ of_list (fst Zs)[<=]lv)
+  -> (forall n Zs a, get F n Zs -> get ans n a -> disj D (defVars Zs a))
+  -> Indexwise.indexwise_R (funConstr D Dt) F ans
+  -> pairwise_ne disj (zip defVars F ans)
+  -> get F n Zs
+  -> get alv n a
+  -> get ans n an
+  -> lv ⊆ D
+  -> exists ϱ1 ϱ2, regAssign (snd Zs) a ϱ1 = Success ϱ2
+             /\ regAssignF regAssign ϱ2 (drop (S n) F) (drop (S n) alv) = Success ϱ'
+             /\ agree_on eq (G \ list_union (zip defVars (take n F) (take n ans)))
+                        (findt (ϱ[fst Zs <-- fresh_list least_fresh
+                                      (SetConstructs.map (findt ϱ 0) (getAnn a \ of_list (fst Zs)))
+                                      (length (fst Zs))]) 0)
+                        (findt ϱ1 0).
+Proof.
+  intros EQ REN LV LVINC DDISJ FUNC PWDISJ GET1 GET2 GET3 incl.
+  general induction GET1; inv GET2; inv GET3; simpl in * |- *; monadS_inv EQ; eauto.
+  - do 2 eexists; split; eauto. split. rewrite EQ0. reflexivity. reflexivity.
+  - exploit (IHGET1 G); hnf; intros; eauto using get; dcr.
+    do 2 eexists; split; eauto. split; eauto.
+    rewrite EQ0. simpl. rewrite EQ1; eauto.
+    etransitivity; eapply agree_on_incl; eauto; try reflexivity.
+    + repeat rewrite <- map_update_list_update_agree; eauto.
+      erewrite least_fresh_list_ext; eauto.
+      eapply update_with_list_agree; eauto.
+      eapply regAssign_renamedApart_agree' in EQ0; eauto using get.
+      rewrite <- map_update_list_update_agree in EQ0; eauto.
+      eapply update_with_list_agree_inv in EQ0; eauto.
+      eapply agree_on_incl; eauto. norm_lunion.
+      instantiate (1:=G \ list_union zip defVars (take n xl) (take n xl1)).
+      unfold defVars at 1. clear_all; cset_tac; intuition.
+      eapply lookup_set_agree; eauto.
+      eapply regAssign_renamedApart_agree' in EQ0; eauto using get.
+      rewrite <- map_update_list_update_agree in EQ0; eauto.
+      eapply update_with_list_agree_inv in EQ0; eauto.
+      eapply agree_on_incl; eauto.
+      instantiate (1:=getAnn a \ of_list (fst x)).
+      setoid_rewrite minus_union at 1.
+      assert (disj (getAnn a \ of_list (fst x)) (snd (getAnn x'1) ∪ of_list (fst x'))). {
+        exploit PWDISJ; [| eauto using get| econstructor 2; eapply zip_get; eauto|].
+        omega. unfold defVars in X.
+        exploit (LVINC (S n)); eauto using get; dcr.
+        rewrite H5. rewrite incl. rewrite union_comm. eapply DDISJ; eauto using get.
+      }
+      setoid_rewrite disj_minus_eq at 2; eauto.
+    + norm_lunion. clear_all; cset_tac; intuition.
+Qed.
+
+Lemma get_take_lt k X (L:list X) n x
+: get (take k L) n x -> n < k.
+Proof.
+  intros. general induction k; destruct L; simpl in *; isabsurd.
+  - inv H; eauto; try omega.
+    + exploit IHk; eauto. omega.
+Qed.
+
+Lemma get_take k X (L:list X) n x
+: get (take k L) n x -> get L n x.
+Proof.
+  intros. general induction k; destruct L; simpl in *; isabsurd.
+  inv H; eauto using get.
+Qed.
+
+Lemma defVars_take_disj F ans n Zs a
+:  pairwise_ne disj (zip defVars F ans)
+   -> get F n Zs
+   -> get ans n a
+   -> disj (defVars Zs a) (list_union zip defVars (take n F) (take n ans)).
+Proof.
+  intros.
+  symmetry. rewrite <- list_union_disjunct; intros.
+  inv_zip H2.
+  eapply H. Focus 3. eapply zip_get; eauto.
+  Focus 2.
+  eapply zip_get; eauto using get_take.
+  exploit get_take_lt; eauto. omega.
+Qed.
+
+Lemma defVars_drop_disj F ans n Zs a
+:  pairwise_ne disj (zip defVars F ans)
+   -> get F n Zs
+   -> get ans n a
+   -> disj (defVars Zs a) (list_union zip defVars (drop (S n) F) (drop (S n) ans)).
+Proof.
+  intros.
+  symmetry. rewrite <- list_union_disjunct; intros.
+  inv_zip H2.
+  eapply H. Focus 3. eapply zip_get; eauto.
+  Focus 2. eapply zip_get; eauto using get_drop. omega.
+Qed.
+
+Lemma defVars_disj_D F ans D Dt D'
+      (D'def:list_union zip defVars F ans ++ Dt[=]D')
+      (Ddisj: disj D D')
+: forall n  DD' Zs, get F n Zs -> get ans n DD' ->
+               disj D (defVars Zs DD').
+Proof.
+  intros.
+  eapply disj_2_incl; eauto. rewrite <- D'def.
+  eapply incl_union_left. eapply incl_list_union; eauto.
+  eapply zip_get; eauto. reflexivity.
+Qed.
+
 (** ** the algorithm produces a locally injective renaming *)
 
-Lemma reg_assign_correct (ϱ:Map [var,var]) LV s alv ϱ' al
+Lemma regAssign_correct (ϱ:Map [var,var]) LV s alv ϱ' al
       (LS:live_sound FunctionalAndImperative LV s alv)
       (inj:injective_on (getAnn alv) (findt ϱ 0))
-      (allocOK:reg_assign s alv ϱ = Success ϱ')
+      (allocOK:regAssign s alv ϱ = Success ϱ')
       (incl:getAnn alv ⊆ fst (getAnn al))
       (sd:renamedApart s al)
 : locally_inj (findt ϱ' 0) s alv.
@@ -109,7 +270,7 @@ Proof.
     + rewrite H9. simpl in *. rewrite <- incl, <- H0.
       clear_all; cset_tac; intuition.
       decide (x === a); eauto.
-    + exploit reg_assign_renamedApart_agree; try eapply allocOK; simpl; eauto using live_sound.
+    + exploit regAssign_renamedApart_agree; try eapply allocOK; simpl; eauto using live_sound.
       rewrite H9 in *.
       simpl in *.
       econstructor. eauto using injective_on_incl.
@@ -119,8 +280,8 @@ Proof.
       etransitivity. eapply map_update_update_agree.
       eapply X0.
       revert H5 incl; clear_all; cset_tac; intuition. invc H0. eauto.
-  - exploit reg_assign_renamedApart_agree; try eapply EQ; simpl; eauto using live_sound.
-    exploit reg_assign_renamedApart_agree; try eapply EQ0; simpl; eauto using live_sound.
+  - exploit regAssign_renamedApart_agree; try eapply EQ; simpl; eauto using live_sound.
+    exploit regAssign_renamedApart_agree; try eapply EQ0; simpl; eauto using live_sound.
     rewrite H11 in X. rewrite H12 in X0.
     simpl in *.
     exploit IHLS1; eauto using injective_on_incl.
@@ -134,7 +295,7 @@ Proof.
     eapply injective_on_agree; eauto. eauto using agree_on_incl.
     eapply locally_inj_live_agree. eauto. eauto. eauto.
     rewrite H11; simpl; eauto.
-    exploit reg_assign_renamedApart_agree'; try eapply EQ0; simpl; eauto using live_sound.
+    exploit regAssign_renamedApart_agree'; try eapply EQ0; simpl; eauto using live_sound.
     rewrite H12 in X3. simpl in *.
     eapply agree_on_incl. eapply X3. instantiate (1:=D ++ Ds).
     pose proof (renamedApart_disj H9). unfold disj in H2.
@@ -149,7 +310,7 @@ Proof.
     + rewrite H10. simpl in *. rewrite <- incl.
       revert H0; clear_all; cset_tac; intuition.
       decide (x === a); eauto. right; eapply H0; cset_tac; intuition.
-    + exploit reg_assign_renamedApart_agree; try eapply allocOK; simpl; eauto using live_sound.
+    + exploit regAssign_renamedApart_agree; try eapply allocOK; simpl; eauto using live_sound.
       rewrite H10 in *.
       simpl in *.
       econstructor. eauto using injective_on_incl.
@@ -159,59 +320,108 @@ Proof.
       etransitivity. eapply map_update_update_agree.
       eapply X0.
       revert H6 incl; clear_all; cset_tac; intuition. invc H0. eauto.
-  - simpl in *.
-    exploit reg_assign_renamedApart_agree; try eapply EQ; simpl; eauto using live_sound.
-    exploit reg_assign_renamedApart_agree; try eapply EQ0; simpl; eauto using live_sound.
-    rewrite <- map_update_list_update_agree in X.
-    exploit IHLS1; eauto.
-    + eapply injective_on_agree; [| eapply map_update_list_update_agree].
-      eapply injective_on_incl.
-      instantiate (1:=getAnn als \ of_list Z ++ of_list Z).
-      eapply injective_on_fresh_list; eauto.
-      eapply injective_on_incl; eauto.
-      rewrite fresh_list_length; eauto.
-      eapply fresh_list_spec. eapply least_fresh_spec.
-      eapply fresh_list_unique, least_fresh_spec.
-      clear_all; cset_tac; intuition.
-      decide (a ∈ of_list Z); intuition.
-      rewrite fresh_list_length; eauto.
-    + rewrite H9. simpl. rewrite <- incl.
-      revert H0; clear_all; cset_tac; intuition.
-      specialize (H0 a). cset_tac; intuition.
-      decide (a ∈ of_list Z); intuition.
-    + assert (injective_on lv (findt ϱ' 0)).
-      eapply injective_on_incl.
-      eapply injective_on_agree; try eapply inj; eauto.
-      etransitivity.
-      eapply agree_on_incl.
-      eapply update_with_list_agree_inv; try eapply X; eauto.
-      rewrite fresh_list_length; eauto.
-      rewrite H9; simpl. rewrite incl.
-      revert H5; clear_all; cset_tac; intuition; eauto.
-      eapply agree_on_incl; eauto. rewrite H12; simpl; eauto. reflexivity.
-      exploit IHLS2; try eapply EQ0; eauto using injective_on_incl.
-      * eapply injective_on_incl.
-        eapply injective_on_agree; try eapply inj; eauto.
+  -
+    exploit regAssign_renamedApart_agreeF; eauto using regAssign_renamedApart_agree'. reflexivity.
+    exploit regAssign_renamedApart_agree; try eapply EQ0; simpl; eauto using live_sound.
+    exploit IHLS; eauto.
+    + eapply injective_on_incl; eauto.
+      eapply injective_on_agree; eauto.
+      eapply agree_on_incl; eauto. instantiate (1:=D).
+      rewrite disj_minus_eq; eauto. simpl in *.
+      symmetry. rewrite <- list_union_disjunct.
+      intros. inv_zip H4. edestruct H8; eauto; dcr.
+      unfold defVars. rewrite meet_comm. eapply disj_app; split; eauto.
+      symmetry; eauto.
+      exploit H7; eauto. eapply renamedApart_disj in X1.
+      eapply disj_1_incl; eauto. rewrite H14. eauto with cset.
+    + pe_rewrite. etransitivity; eauto.
+    +
+      assert (DDISJ:forall n  DD' Zs, get F n Zs -> get ans n DD' ->
+                              disj D (defVars Zs DD')).
+      {
+        eapply renamedApart_disj in sd. eauto using defVars_disj_D.
+      }
+
+      econstructor; eauto.
+      * intros. edestruct get_length_eq; try eapply H6; eauto.
+        edestruct (regAssignF_get (fst (getAnn x0) ++ snd (getAnn x0) ++ getAnn alv)); eauto; dcr.
+        rewrite <- map_update_list_update_agree in H18; eauto.
+        exploit H1; try eapply H16; eauto.
+        assert (getAnn alv \ of_list (fst Zs) ++ of_list (fst Zs) [=] getAnn alv).
+        edestruct H2; eauto. revert H14; clear_all; cset_tac; intuition.
+        decide (a ∈ of_list (fst Zs)); eauto.
+        eapply injective_on_agree.
+        Focus 2.
         eapply agree_on_incl.
-        eapply update_with_list_agree_inv; try eapply X; eauto.
-        rewrite fresh_list_length; eauto.
-        rewrite H9; simpl. rewrite incl.
-        revert H5; clear_all; cset_tac; intuition; eauto. eauto.
-      * rewrite H12. simpl. simpl in *. rewrite <- incl. eauto.
-      * econstructor; eauto.
-        eapply locally_inj_live_agree; eauto.
-        rewrite H9. simpl.
-        eapply agree_on_incl.
-        eapply reg_assign_renamedApart_agree'; try eapply EQ0; eauto.
-        rewrite H12; simpl. instantiate (1:=(of_list Z ++ D) ++ Ds).
-        pose proof (renamedApart_disj sd). unfold disj in H3.
-        simpl in *. rewrite <- H7 in H3.
-        revert H5 H6 H3; clear_all; cset_tac; intuition eauto; eauto.
-        rewrite H9. simpl. rewrite <- incl.
-        revert H0; clear_all; cset_tac; intuition.
-        specialize (H0 a). cset_tac; intuition.
-        decide (a ∈ of_list Z); intuition.
-    + rewrite fresh_list_length; eauto.
+        eauto. do 2 rewrite <- incl_right.
+        rewrite disj_minus_eq; eauto.
+        eapply renamedApart_disj in sd.
+        simpl in *.
+        rewrite <- H14. symmetry. rewrite disj_app. split; symmetry.
+        eapply disj_1_incl. eapply disj_2_incl. eapply sd.
+        rewrite <- H13. eapply incl_union_left.
+        hnf; intros. eapply list_union_get in H17. destruct H17. dcr.
+        inv_zip H17.
+        eapply incl_list_union. eapply zip_get.
+        eapply get_take; eauto. eauto using get_take. reflexivity. eauto.
+        cset_tac; intuition.
+        edestruct H2; eauto; dcr. rewrite <- incl. eauto.
+        eapply disj_1_incl.
+        eapply defVars_take_disj; eauto. unfold defVars.
+        eauto with cset.
+        setoid_rewrite <- H14 at 1.
+        eapply injective_on_fresh_list; eauto.
+        eapply injective_on_incl; eauto.
+        eapply H2; eauto.
+        eapply disj_2_incl. eapply fresh_list_spec. eapply least_fresh_spec.
+        reflexivity.
+        edestruct H8; eauto.
+        eapply fresh_list_unique, least_fresh_spec.
+        edestruct H8; eauto; dcr. rewrite H14.
+        exploit H2; eauto; dcr. rewrite incl in H20.
+        revert H20; clear_all; cset_tac; intuition.
+        decide (a ∈ of_list (fst Zs)); intuition.
+        eapply locally_inj_live_agree; try eapply X2; eauto.
+        eapply regAssign_renamedApart_agreeF in H15;
+          eauto using regAssign_renamedApart_agree', get_drop, drop_length_stable; try reflexivity.
+        eapply regAssign_renamedApart_agree' in EQ0; simpl; eauto using live_sound.
+        etransitivity; eapply agree_on_incl; eauto.
+        rewrite disj_minus_eq. reflexivity.
+        {
+          edestruct H8; eauto; dcr. rewrite H14.
+          rewrite union_comm. rewrite <- union_assoc.
+          symmetry; rewrite disj_app; split; symmetry.
+          - eapply disj_1_incl. eapply defVars_drop_disj; eauto.
+            unfold defVars. eauto with cset.
+          - eapply renamedApart_disj in sd; simpl in sd.
+            eapply disj_2_incl; eauto.
+            rewrite <- H13. eapply incl_union_left.
+            rewrite <- drop_zip; eauto.
+            eapply list_union_drop_incl; eauto.
+        }
+        pe_rewrite.
+        rewrite disj_minus_eq. reflexivity.
+        {
+          edestruct H8; eauto; dcr. rewrite H14.
+          rewrite union_comm. rewrite <- union_assoc.
+          symmetry; rewrite disj_app; split; symmetry.
+          rewrite union_comm; eauto.
+          eapply renamedApart_disj in H10. pe_rewrite. eapply H10.
+        }
+        edestruct H8; eauto; dcr. rewrite H14.
+        exploit H2; eauto; dcr. rewrite incl in H20.
+        revert H20; clear_all; cset_tac; intuition.
+        decide (a ∈ of_list (fst Zs)); intuition.
+      * eapply injective_on_agree; try eapply inj; eauto.
+        etransitivity; eapply agree_on_incl; eauto.
+        rewrite disj_minus_eq; eauto. simpl in *.
+        symmetry. rewrite <- list_union_disjunct.
+        intros. inv_zip H4. edestruct H8; eauto; dcr.
+        unfold defVars. rewrite meet_comm. eapply disj_app; split; eauto.
+        symmetry; eauto.
+        exploit H7; eauto. eapply renamedApart_disj in X2.
+        eapply disj_1_incl; eauto. rewrite H14. eauto with cset.
+        pe_rewrite. eauto.
 Qed.
 
 
@@ -220,22 +430,22 @@ Require Import Restrict RenamedApart_Liveness.
 (** ** Theorem 8 from the paper. *)
 (** One could prove this theorem directly by induction, however, we exploit that
     under the assumption of the theorem, the liveness information [alv] is also
-    sound for functional liveness and we can thus rely on theorem [reg_assign_correct]
+    sound for functional liveness and we can thus rely on theorem [regAssign_correct]
     above, which we did prove by induction. *)
 
-Lemma reg_assign_correct' s ang ϱ ϱ' (alv:ann (set var)) Lv
+Lemma regAssign_correct' s ang ϱ ϱ' (alv:ann (set var)) Lv
   : renamedApart s ang
   -> live_sound Imperative Lv s alv
   -> bounded (live_globals Lv) (fst (getAnn ang))
   -> ann_R Subset1 alv ang
   -> LabelsDefined.noUnreachableCode s
   -> injective_on (getAnn alv) (findt ϱ 0)
-  -> reg_assign s alv ϱ = Success ϱ'
+  -> regAssign s alv ϱ = Success ϱ'
   -> locally_inj (findt ϱ' 0) s alv.
 Proof.
   intros.
   eapply renamedApart_live_imperative_is_functional in H0; eauto using bounded_disjoint, renamedApart_disj, meet1_Subset1, live_sound_annotation, renamedApart_annotation.
-  eapply reg_assign_correct; eauto using locally_inj_subset, meet1_Subset, live_sound_annotation, renamedApart_annotation.
+  eapply regAssign_correct; eauto using locally_inj_subset, meet1_Subset, live_sound_annotation, renamedApart_annotation.
   eapply ann_R_get in H2. destruct (getAnn ang); simpl; cset_tac; intuition.
 Qed.
 
@@ -248,14 +458,40 @@ Fixpoint largest_live_set (a:ann (set var)) : set var :=
     | ann0 gamma => gamma
     | ann1 gamma a => max_set gamma (largest_live_set a)
     | ann2 gamma a b => max_set gamma (max_set (largest_live_set a) (largest_live_set b))
+    | annF gamma s b => max_set gamma (max_set (fold_left (fun gamma b => max_set gamma (largest_live_set b)) s ∅)
+                                      (largest_live_set b))
   end.
+
+Notation "'list_max' L" := (fold_left max L 0) (at level 50).
+
+Lemma list_max_swap L x
+: max (list_max L) x = fold_left max L x.
+Proof.
+  general induction L; simpl; eauto.
+  setoid_rewrite <- IHL; eauto.
+  setoid_rewrite NPeano.Nat.max_comm at 4.
+  rewrite NPeano.Nat.max_assoc; eauto.
+Qed.
+
+Lemma list_max_get L n x
+: get L n x
+  -> x <= list_max L.
+Proof.
+  intros. general induction L; eauto; invt get; simpl.
+  - rewrite <- list_max_swap. eapply Max.le_max_r.
+  - rewrite <- list_max_swap. rewrite <- Max.le_max_l; eauto.
+Qed.
 
 Fixpoint size_of_largest_live_set (a:ann (set var)) : nat :=
   match a with
     | ann0 gamma => SetInterface.cardinal gamma
     | ann1 gamma a => max (SetInterface.cardinal gamma) (size_of_largest_live_set a)
     | ann2 gamma a b => max (SetInterface.cardinal gamma)
-                       (max (size_of_largest_live_set a) (size_of_largest_live_set b))
+                       (max (size_of_largest_live_set a)
+                            (size_of_largest_live_set b))
+    | annF gamma a b => max (SetInterface.cardinal gamma)
+                       (max (list_max (List.map size_of_largest_live_set a))
+                            (size_of_largest_live_set b))
   end.
 
 Lemma size_of_largest_live_set_live_set al
@@ -264,20 +500,20 @@ Proof.
   destruct al; simpl; eauto using Max.le_max_l.
 Qed.
 
-Lemma reg_assign_assignment_small (ϱ:Map [var,var]) LV s alv ϱ' al n
+Lemma regAssign_assignment_small (ϱ:Map [var,var]) LV s alv ϱ' al n
       (LS:live_sound Functional LV s alv)
-      (allocOK:reg_assign s alv ϱ = Success ϱ')
+      (allocOK:regAssign s alv ϱ = Success ϱ')
       (incl:getAnn alv ⊆ fst (getAnn al))
       (sd:renamedApart s al)
       (up:lookup_set (findt ϱ 0) (fst (getAnn al)) ⊆ vars_up_to n)
 : lookup_set (findt ϱ' 0) (snd (getAnn al)) ⊆ vars_up_to (max (size_of_largest_live_set alv) n).
 Proof.
-  exploit reg_assign_renamedApart_agree; eauto using live_sound.
+  exploit regAssign_renamedApart_agree; eauto using live_sound.
   rewrite lookup_set_agree in up; eauto. clear X.
   general induction LS; invt renamedApart; simpl in * |- *.
   - assert ( singleton (findt ϱ' 0 x)
                        ⊆ vars_up_to (size_of_largest_live_set al)). {
-      eapply reg_assign_renamedApart_agree in allocOK; eauto.
+      eapply regAssign_renamedApart_agree in allocOK; eauto.
       rewrite <- allocOK. unfold findt at 1.
       rewrite MapFacts.add_eq_o; eauto.
       cset_tac. invc H2. eapply in_vars_up_to.
@@ -310,34 +546,32 @@ Proof.
       repeat rewrite vars_up_to_max.
       cset_tac; intuition; eauto.
   - monadS_inv allocOK.
-    exploit IHLS1; eauto.
-    rewrite H11; eauto. simpl. rewrite <- incl; eauto.
-    rewrite H11; simpl.
-    rewrite lookup_set_agree; eauto.
-    eapply agree_on_incl; try eapply reg_assign_renamedApart_agree;
-    try eapply EQ0; eauto using live_sound.
-    rewrite H12; simpl; eauto.
-    exploit IHLS2; try eapply EQ0; eauto.
-    rewrite H12; simpl. rewrite <- incl; eauto.
-    rewrite H12. simpl. eauto.
-    rewrite H11 in X; rewrite H12 in X0. simpl in *.
-    rewrite <- H7.
-    rewrite lookup_set_union; eauto.
-    rewrite X0.
-    rewrite lookup_set_agree; eauto. rewrite X.
-    repeat (try rewrite <- NPeano.Nat.add_max_distr_r; rewrite vars_up_to_max).
-    clear_all; cset_tac; intuition.
-    unfold findt; intuition.
-    unfold findt; intuition.
-    eapply agree_on_incl.
-    symmetry.
-    eapply reg_assign_renamedApart_agree'; try eapply EQ0; eauto. rewrite H12; simpl.
-    instantiate (1:=Ds). revert H6; clear_all; cset_tac; intuition; eauto.
+    exploit IHLS1; eauto; pe_rewrite.
+    + rewrite <- incl; eauto.
+    + rewrite lookup_set_agree; eauto.
+      eapply agree_on_incl; try eapply regAssign_renamedApart_agree;
+      try eapply EQ0; eauto using live_sound.
+      rewrite H12; simpl; eauto.
+    + exploit IHLS2; try eapply EQ0; eauto; pe_rewrite.
+      * rewrite <- incl; eauto.
+      * simpl. eauto.
+      * rewrite <- H7.
+        rewrite lookup_set_union; eauto.
+        rewrite X0.
+        rewrite lookup_set_agree; eauto. rewrite X.
+        repeat (try rewrite <- NPeano.Nat.add_max_distr_r; rewrite vars_up_to_max).
+        clear_all; cset_tac; intuition.
+        unfold findt; intuition.
+        unfold findt; intuition.
+        eapply agree_on_incl.
+        symmetry.
+        eapply regAssign_renamedApart_agree'; try eapply EQ0; eauto. rewrite H12; simpl.
+        instantiate (1:=Ds). revert H6; clear_all; cset_tac; intuition; eauto.
   - rewrite H7. rewrite lookup_set_empty; cset_tac; intuition; eauto.
   - rewrite H2. rewrite lookup_set_empty; cset_tac; intuition; eauto.
   - assert ( singleton (findt ϱ' 0 x)
                        ⊆ vars_up_to (size_of_largest_live_set al)). {
-      eapply reg_assign_renamedApart_agree in allocOK; eauto.
+      eapply regAssign_renamedApart_agree in allocOK; eauto.
       rewrite <- allocOK. unfold findt at 1.
       rewrite MapFacts.add_eq_o; eauto.
       cset_tac. invc H2. eapply in_vars_up_to.
@@ -368,118 +602,190 @@ Proof.
       rewrite H11. rewrite lookup_set_add, X; eauto.
       repeat rewrite vars_up_to_max.
       cset_tac; intuition.
-  - monadS_inv allocOK.
-    simpl in *.
-    exploit reg_assign_renamedApart_agree; try eapply EQ; simpl; eauto using live_sound.
-    exploit reg_assign_renamedApart_agree; try eapply EQ0; simpl; eauto using live_sound.
-    rewrite H9 in *. rewrite H12 in *. simpl in *.
-    assert (D [=] (of_list Z ++ D) \ of_list Z). {
-      revert H5. clear_all; cset_tac; intuition.
-      specialize (H0 a). intuition.
-    }
-   assert (SetInterface.cardinal
-             (SetConstructs.map (findt ϱ 0) (getAnn als \ of_list Z)) +
-           length Z <= size_of_largest_live_set als). {
-      rewrite cardinal_map.
-      rewrite <- size_of_largest_live_set_live_set.
-      exploit (diff_inter_cardinal (getAnn als) (of_list Z)).
-      assert (getAnn als ∩ of_list Z [=] of_list Z).
-      revert H; clear_all; cset_tac; intuition.
-      rewrite H3 in X1. simpl in *.
-      rewrite <- X1.
-      rewrite cardinal_of_list_unique. omega. eauto. eauto.
-    }
-    rewrite <- map_update_list_update_agree in X.
-    assert (agree_on eq D (findt ϱ 0) (findt ϱ' 0)). etransitivity; eauto.
-    eapply update_with_list_agree_inv in X; try eapply X; eauto.
-    rewrite <- H2 in X; eauto. rewrite fresh_list_length; eauto.
-    exploit IHLS1; eauto.
-    + rewrite H9. simpl. rewrite <- incl.
-      revert H0; clear_all; cset_tac; intuition.
-      specialize (H0 a). cset_tac; intuition.
-      decide (a ∈ of_list Z); intuition.
-    + rewrite H9. simpl.
-      instantiate (1:=(max (size_of_largest_live_set als) n)).
-      rewrite <- lookup_set_agree; try eapply X; eauto.
-      rewrite lookup_set_update_with_list_in_union_length; eauto.
-      rewrite <- H2.
-      rewrite lookup_set_agree; try eapply H3; eauto.
-      rewrite up.
-      repeat (try rewrite <- NPeano.Nat.add_max_distr_r; rewrite vars_up_to_max).
-      rewrite least_fresh_list_small_vars_up_to.
-      intros.
-      rewrite (vars_up_to_incl H3).
-      cset_tac; intuition.
-      rewrite fresh_list_length; eauto.
-    + exploit IHLS2; eauto.
-      * rewrite H12. simpl. simpl in *. rewrite <- incl. eauto.
-      * instantiate (1:=(max (size_of_largest_live_set alb) n)).
-        rewrite H9 in X1. simpl in *.
-        rewrite H12 in *. simpl in *.
-        rewrite up.
-        repeat (try rewrite <- NPeano.Nat.add_max_distr_r; rewrite vars_up_to_max).
-        eauto.
-      * rewrite H9 in X1. rewrite H12 in X2.
-        simpl in *.
-        rewrite <- H7. repeat rewrite lookup_set_union; eauto.
-        rewrite X2. rewrite lookup_set_agree; eauto. rewrite X1.
-        repeat (try rewrite <- NPeano.Nat.add_max_distr_r; rewrite vars_up_to_max).
-        erewrite lookup_set_agree with (m':=
-          MapUpdate.update_with_list Z (fresh_list least_fresh
-                                       (SetConstructs.map (findt ϱ 0) (getAnn als \ of_list Z))
-                                       (length Z))
-                                     (findt ϱ 0)); eauto.
-        rewrite update_with_list_lookup_set_incl; eauto.
+  - repeat (try rewrite <- NPeano.Nat.add_max_distr_r; rewrite vars_up_to_max).
+    monadS_inv allocOK.
+    rewrite <- H13, lookup_set_union; eauto.
+    eapply union_incl_split.
+    + rewrite lookup_set_list_union; [ | eauto | eapply lookup_set_empty; eauto ].
+      eapply list_union_incl; intros; eauto with cset.
+      assert (DDISJ:forall n  DD' Zs, get F n Zs -> get ans n DD' ->
+                              disj D (defVars Zs DD')).
+      {
+        intros. eapply renamedApart_disj in sd; simpl in *.
+        eapply disj_2_incl; eauto. rewrite <- H13.
+        eapply incl_union_left. eapply incl_list_union; eauto.
+        eapply zip_get; eauto. reflexivity.
+      }
+      inv_map H4. inv_zip H5. edestruct get_length_eq; try eapply H; eauto.
+      edestruct regAssignF_get; eauto; dcr.
+      edestruct H2; eauto.
+      edestruct H8; eauto; dcr.
+      exploit H1; eauto.
+      rewrite H22. rewrite <- incl.
+      revert H20. clear_all; cset_tac; intuition.
+      decide (a ∈ of_list (fst x1)); intuition.
+      rewrite H22. instantiate (1:=max (list_max List.map size_of_largest_live_set als) n).
+      rewrite lookup_set_union; eauto.
+      eapply union_incl_split.
+      {
+        rewrite <- map_update_list_update_agree in H21; eauto.
+        exploit regAssign_renamedApart_agree'; try eapply H19; eauto.
+        rewrite <- lookup_set_agree.
+        Focus 4. etransitivity; eapply agree_on_incl. eapply H21.
+        rewrite disj_minus_eq; [ | eauto using defVars_take_disj].
+        unfold defVars. eauto. eauto.
+        rewrite disj_minus_eq; eauto.
+        exploit H7; eauto. eapply renamedApart_disj in X0.
+        eapply disj_1_incl; eauto. rewrite H22.
+        rewrite <- incl. revert H20.
+        clear_all; cset_tac; intuition.
+        decide (a ∈ of_list (fst x1)); intuition.
+        rewrite lookup_set_update_with_list_in_union_length; eauto.
+        rewrite diff_subset_equal. rewrite lookup_set_empty.
         rewrite least_fresh_list_small_vars_up_to.
-        rewrite (vars_up_to_incl H3).
-        cset_tac; intuition.
-        rewrite fresh_list_length; eauto.
+        eapply union_incl_split; eauto. clear_all; cset_tac; intuition.
+        eapply vars_up_to_incl.
+        rewrite cardinal_map; eauto.
+        rewrite cardinal_difference'.
+        rewrite cardinal_of_list_unique; eauto.
+        etransitivity; [|eapply Max.le_max_l].
+        assert (length (fst x1) <= SetInterface.cardinal (getAnn x0)).
+        rewrite <- (diff_inter_cardinal (getAnn x0) (of_list (fst x1))).
+        assert (getAnn x0 ∩ of_list (fst x1) [=] of_list (fst x1)).
+        revert H17; clear_all; cset_tac; intuition.
+        rewrite H23 at 1. rewrite cardinal_of_list_unique; eauto. omega.
+        etransitivity;[| eapply list_max_get; eauto; eapply map_get_1; eauto].
+        rewrite <- size_of_largest_live_set_live_set. omega.
+        eauto. intuition. eauto. intuition. intuition.
+      }
+      {
+        exploit regAssign_renamedApart_agreeF; eauto using drop_get, get_drop, drop_length_stable,
+                                               regAssign_renamedApart_agree'. reflexivity.
+        rewrite vars_up_to_max. eapply incl_union_right.
+        exploit regAssign_renamedApart_agree'; try eapply EQ0; eauto.
+        rewrite lookup_set_agree; try eapply up; intuition.
+        etransitivity; eapply agree_on_incl; eauto.
+        instantiate (1:=D). rewrite disj_minus_eq; eauto.
+        eapply renamedApart_disj in sd.
+        eapply disj_2_incl. eauto.
+        unfold getAnn, snd. rewrite <- H13.
+        eapply incl_union_left.
+        rewrite <- drop_zip.
+        eapply list_union_drop_incl; eauto. congruence.
+        instantiate (1:=D). pe_rewrite.
+        eapply renamedApart_disj in H10. pe_rewrite.
+        rewrite disj_minus_eq; eauto.
+      }
+      unfold defVars. rewrite lookup_set_union; eauto.
+      eapply union_incl_split.
+      * assert (FLEQ:lookup_set (findt ϱ' 0) (of_list (fst x1)) ⊆
+                           of_list (fresh_list least_fresh
+                                               (SetConstructs.map (findt ϱ 0) (getAnn x0 \ of_list (fst x1)))
+                                               (length (fst x1)))).
+        {
+          rewrite <- map_update_list_update_agree in H21; eauto.
+          exploit regAssign_renamedApart_agreeF; eauto using drop_get, get_drop, drop_length_stable,
+                                                 regAssign_renamedApart_agree'. reflexivity.
+          exploit regAssign_renamedApart_agree'; try eapply EQ0; eauto.
+          exploit regAssign_renamedApart_agree'; eauto.
+          rewrite <- lookup_set_agree.
+          Focus 4.
+          etransitivity; [| eapply agree_on_incl; try eapply X1].
+          etransitivity; [| eapply agree_on_incl; try eapply X0].
+          etransitivity; [| eapply agree_on_incl; try eapply X2].
+          eapply agree_on_incl; try apply H21.
+          rewrite disj_minus_eq; [ | eauto using defVars_take_disj].
+          unfold defVars. eapply incl_left.
+          rewrite disj_minus_eq; eauto.
+          exploit H7; eauto. eapply renamedApart_disj in X3.
+          eapply disj_1_incl; eauto. rewrite H22.
+          rewrite <- incl. revert H20. clear_all; cset_tac; intuition.
+          decide (a ∈ of_list (fst x1)); intuition.
+          rewrite disj_minus_eq; [ | eauto using defVars_drop_disj].
+          eapply incl_left.
+          rewrite disj_minus_eq; eauto.
+          pe_rewrite.
+          assert (getAnn x0 [=] getAnn x0 \ of_list (fst x1) ∪ of_list (fst x1)).
+          revert H17; clear_all; cset_tac; intuition.
+          decide (a ∈ of_list (fst x1)); eauto. rewrite H23.
+          symmetry. eapply disj_app; split. symmetry.
+          eapply disj_1_incl. eapply disj_2_incl.
+          eapply renamedApart_disj in sd. eapply sd. simpl.
+          rewrite <- H13. eapply incl_right.
+          simpl. rewrite H20; eauto.
+          symmetry.
+          eapply renamedApart_disj in H10. pe_rewrite.
+          eapply disj_1_incl; eauto. eapply incl_left.
+          rewrite lookup_set_update_with_list_in_union_length; eauto.
+          rewrite diff_subset_equal. rewrite lookup_set_empty.
+          clear_all; cset_tac; intuition. intuition. reflexivity.
+          intuition. intuition.
+        }
+        rewrite FLEQ.
+        rewrite least_fresh_list_small_vars_up_to.
+        eapply incl_union_left. eapply incl_union_right.
+        eapply incl_union_left.
+        eapply vars_up_to_incl.
+        rewrite cardinal_map; eauto.
+        rewrite cardinal_difference'.
+        rewrite cardinal_of_list_unique; eauto.
+        assert (length (fst x1) <= SetInterface.cardinal (getAnn x0)).
+        rewrite <- (diff_inter_cardinal (getAnn x0) (of_list (fst x1))).
+        assert (getAnn x0 ∩ of_list (fst x1) [=] of_list (fst x1)).
+        revert H17; clear_all; cset_tac; intuition.
+        rewrite H23 at 1. rewrite cardinal_of_list_unique; eauto. omega.
+        etransitivity;[| eapply list_max_get; eauto; eapply map_get_1; eauto].
+        rewrite <- size_of_largest_live_set_live_set. omega.
+        eauto.
+      * erewrite lookup_set_agree; eauto. erewrite X; eauto.
+        repeat (try rewrite <- NPeano.Nat.add_max_distr_r; rewrite vars_up_to_max); eauto.
+        setoid_rewrite vars_up_to_incl at 1. instantiate (1:=list_max List.map size_of_largest_live_set als).
+        clear_all; cset_tac; intuition.
+        eapply list_max_get. eapply map_get_1; eauto.
+        eapply regAssign_renamedApart_agree' in EQ0; eauto. symmetry in EQ0.
+        etransitivity; eapply agree_on_incl; eauto.
+        pe_rewrite. rewrite disj_minus_eq. reflexivity. eauto with cset.
         symmetry.
-        etransitivity.
-        eapply agree_on_incl.
-        rewrite map_update_list_update_agree.
-        eapply reg_assign_renamedApart_agree'; try eapply EQ; eauto.
-        rewrite fresh_list_length; eauto.
-        instantiate (1:=of_list Z). rewrite H9. simpl.
-        generalize (renamedApart_disj H8).
-        rewrite H9. simpl. unfold disj. clear_all; cset_tac; intuition; eauto.
-        eapply agree_on_incl.
-        eapply reg_assign_renamedApart_agree'; try eapply EQ0; eauto.
-        instantiate (1:=of_list Z). rewrite H12. simpl.
-        revert H6. clear_all; cset_tac; intuition; eauto.
-        symmetry.
-        eapply agree_on_incl.
-        eapply reg_assign_renamedApart_agree'; try eapply EQ0; eauto.
-        instantiate (1:=Ds). rewrite H12. simpl.
-        revert H6; clear_all; cset_tac; intuition; eauto.
-    + rewrite fresh_list_length; eauto.
+        eapply regAssign_renamedApart_agreeF; intros; eauto using get_drop, drop_length_stable.
+        eapply regAssign_renamedApart_agree'; eauto using get_drop. reflexivity.
+        rewrite disj_minus_eq. reflexivity.
+        eapply disj_1_incl. eapply defVars_drop_disj; eauto. unfold defVars.
+        eauto with cset.
+    + exploit IHLS; eauto.
+      * pe_rewrite. rewrite <- incl; eauto.
+      * pe_rewrite. instantiate (1:=max (list_max (List.map size_of_largest_live_set als)) n).
+        repeat (try rewrite <- NPeano.Nat.add_max_distr_r; rewrite vars_up_to_max).
+        rewrite up; eauto with cset.
+      * pe_rewrite.
+        repeat (try rewrite <- NPeano.Nat.add_max_distr_r in X; rewrite vars_up_to_max in X).
+        rewrite X. clear_all; cset_tac; intuition.
 Qed.
 
 (** ** Theorem 8 from the paper. *)
 (** One could prove this theorem directly by induction, however, we exploit that
     under the assumption of the theorem, the liveness information [alv] is also
-    sound for functional liveness and we can thus rely on theorem [reg_assign_assignment_small]
+    sound for functional liveness and we can thus rely on theorem [regAssign_assignment_small]
     above, which we did prove by induction. *)
 
 
-Lemma reg_assign_assignment_small' s ang ϱ ϱ' (alv:ann (set var)) Lv n
+Lemma regAssign_assignment_small' s ang ϱ ϱ' (alv:ann (set var)) Lv n
   : renamedApart s ang
   -> live_sound Imperative Lv s alv
   -> bounded (live_globals Lv) (fst (getAnn ang))
   -> ann_R Subset1 alv ang
   -> LabelsDefined.noUnreachableCode s
-  -> reg_assign s alv ϱ = Success ϱ'
+  -> regAssign s alv ϱ = Success ϱ'
   -> lookup_set (findt ϱ 0) (fst (getAnn ang)) ⊆ vars_up_to n
   -> lookup_set (findt ϱ' 0) (fst (getAnn ang) ∪ snd (getAnn ang)) ⊆ vars_up_to (max (size_of_largest_live_set alv) n).
 Proof.
   intros.
   eapply renamedApart_live_imperative_is_functional in H0; eauto using bounded_disjoint, renamedApart_disj, meet1_Subset1, live_sound_annotation, renamedApart_annotation.
   eapply live_sound_overapproximation_F in H0.
-  exploit reg_assign_assignment_small; eauto using locally_inj_subset, meet1_Subset, live_sound_annotation, renamedApart_annotation.
+  exploit regAssign_assignment_small; eauto using locally_inj_subset, meet1_Subset, live_sound_annotation, renamedApart_annotation.
   eapply ann_R_get in H2. destruct (getAnn ang); simpl; cset_tac; intuition.
   rewrite lookup_set_union; intuition.
   rewrite X.
-  rewrite <- lookup_set_agree; eauto using reg_assign_renamedApart_agree; intuition.
+  rewrite <- lookup_set_agree; eauto using regAssign_renamedApart_agree; intuition.
   rewrite H5. repeat rewrite vars_up_to_max. cset_tac; intuition.
 Qed.
 
