Fresh.v
@@ -57,10 +57,19 @@ Section SafeFirst.
 
   Hypothesis comp  : forall n, Computable (P n).
 
+  Lemma safe_upward n
+  : safe n -> ~ P n -> safe (S n).
+  Proof.
+    intros; destruct H.
+    - destruct (H0 H).
+    - eapply H.
+  Defined.
+
   Fixpoint safe_first n (s:safe n) : nat.
   refine (if [ P n ] then n else safe_first (S n) _).
-  inv s; eauto; isabsurd.
+  destruct s; eauto. destruct (_H H).
   Defined.
+
 
   Fixpoint safe_first_spec n s
   : P (@safe_first n s).
@@ -72,6 +81,21 @@ Section SafeFirst.
   Qed.
 
 End SafeFirst.
+
+Fixpoint safe_first_ext P Q n
+      (PC:forall n, Computable (P n))
+      (QC:forall n, Computable (Q n))
+      (PS:safe P n)
+      (QS:safe Q n)
+      (EXT:(forall x, P x <-> Q x)) {struct PS}
+: safe_first PC PS = safe_first QC QS.
+Proof.
+  destruct PS; destruct QS; simpl.
+  - destruct (decision_procedure (P n)), (decision_procedure (Q n)); eauto; intuition.
+  - destruct if; destruct (decision_procedure (P n)); eauto; intuition. exfalso; firstorder.
+  - destruct if; destruct (decision_procedure (Q n)); eauto; intuition. exfalso; firstorder.
+  - repeat destruct if; intuition; exfalso; firstorder.
+Qed.
 
 Lemma safe_impl (P Q: nat -> Prop) n
 : safe P n -> (forall x, P x -> Q x) -> safe Q n.
@@ -164,6 +188,17 @@ Definition least_fresh (lv:set var) : var.
     intros. omega. eapply le_is_le; omega.
 Defined.
 
+Lemma least_fresh_ext (G G':set var)
+: G [=] G'
+  -> least_fresh G = least_fresh G'.
+Proof.
+  intros. unfold least_fresh.
+  eapply safe_first_ext; eauto.
+  split; intros.
+  - rewrite <- H; eauto.
+  - rewrite H; eauto.
+Qed.
+
 Lemma least_fresh_full_spec G
 : least_fresh G ∉ G /\ least_fresh G <= cardinal G.
 Proof.
@@ -209,6 +244,12 @@ Section FreshList.
     general induction n; eauto. simpl. f_equal; eauto.
   Qed.
 
+  Lemma fresh_list_length2 (G:set var) n
+  : n = length (fresh_list G n).
+  Proof.
+    general induction n; eauto. simpl. f_equal; eauto.
+  Qed.
+
   Hypothesis fresh_spec : forall G, fresh G ∉ G.
 
   Definition fresh_set (G:set var) (n:nat) : set var :=
@@ -241,6 +282,7 @@ Section FreshList.
   Qed.
 End FreshList.
 
+Hint Resolve fresh_list_length fresh_list_length2.
 
 Lemma least_fresh_list_small G n
 : forall i x, get (fresh_list least_fresh G n) i x -> x < cardinal G + n.
@@ -251,6 +293,16 @@ Proof.
     erewrite cardinal_2 with (s:=G) in X. omega.
     eapply least_fresh_spec.
     hnf; cset_tac; intuition.
+Qed.
+
+Lemma least_fresh_list_ext n G G'
+: G [=] G'
+  -> fresh_list least_fresh G n = fresh_list least_fresh G' n.
+Proof.
+  intros. general induction n; simpl; eauto.
+  f_equal; eauto using least_fresh_ext.
+  erewrite least_fresh_ext; eauto. eapply IHn.
+  rewrite H; eauto.
 Qed.
 
 Fixpoint vars_up_to (n:nat) :=
@@ -314,7 +366,6 @@ Lemma inverse_on_update_fresh_list (D:set var) (Z:list var) (ϱ ϱ' : var -> var
 Proof.
   intros. eapply inverse_on_update_fresh; eauto.
   eapply fresh_list_unique, fresh_spec.
-  rewrite fresh_list_length; eauto.
   eapply fresh_list_spec, fresh_spec.
 Qed.
 
